fairness/examples/comp/lib_ext.v
@@ -1,0 +1,126 @@
+From iris.proofmode Require Import tactics.
+From trillium.fairness.ext_models Require Import ext_models. 
+From trillium.fairness Require Import lm_fair fuel_ext.
+From trillium.fairness.examples.comp Require Import lib. 
+
+Close Scope Z_scope.
+
+
+Section ExtModelInner.
+
+  (* TODO: try to find an appropriate definition for functional relations,
+       try to remove duplication between function and relation
+       (maybe change ETs definition?) *)
+  Definition reset_st_impl (st: fmstate lib_model_impl): fmstate lib_model_impl := 1. 
+  
+  Definition reset_st (st: fmstate lib_model_impl): option (fmstate lib_model_impl) :=
+    if (decide (st = 0)) then Some (reset_st_impl st) else None.
+  Definition reset_st_rel: relation (fmstate lib_model_impl) :=
+    fun x y => reset_st x = Some y. 
+
+  Definition lib_EI := unit.     
+  Definition lib_ETs (ι: lib_EI) := reset_st_rel.
+
+  (* TODO: avoid duplication *)
+  Definition lib_active_exts (st: fmstate lib_model_impl): gset lib_EI := 
+    if (decide (st = 0)) then {[ () ]} else ∅. 
+  
+  Lemma lib_active_exts_spec st ι:
+    ι ∈ lib_active_exts st <-> ∃ st', lib_ETs ι st st'.
+  Proof using.  
+    rewrite /lib_active_exts /lib_ETs /reset_st_rel /reset_st.
+    destruct st; [erewrite !decide_True | erewrite !decide_False]; set_solver.
+  Qed. 
+
+  Instance ExtLib: ExtModel lib_model_impl := 
+    Build_ExtModel lib_model_impl _ _ _ _ _ lib_active_exts_spec.
+
+End ExtModelInner.
+
+Section ExtModelLM.
+
+  Definition lm_is_stopped (ρlg: fmrole lib_fair) (δ: fmstate lib_fair) := 
+    ls_under δ = 0 /\ (* TODO: get rid of this duplication *)
+    ρl ∉ dom (ls_mapping δ) /\
+    ρlg ∈ dom (ls_tmap δ (LM := lib_model)).
+
+  (* TODO: implement it via ls_tmap*)
+  Definition reset_lm_st_impl 
+    (ρlg: fmrole lib_fair) (δ: fmstate lib_fair)
+    (STOP: lm_is_stopped ρlg δ): fmstate lib_fair.
+    refine 
+      {| ls_under := reset_st_impl (ls_under δ); 
+        ls_mapping := <[ρl := ρlg]> (ls_mapping δ);
+        ls_fuel := <[ρl := lm_fl lib_model δ]> (ls_fuel δ) |}.
+    - (* TODO: merge model files, get rid of this *)
+      Transparent lib_model_impl. 
+      set_solver.
+    - rewrite !dom_insert_L. by rewrite ls_same_doms.
+    - done.
+  Defined.       
+
+  Definition reset_lm_st (ρlg: fmrole lib_fair) (δ: fmstate lib_fair): option (fmstate lib_fair) :=
+    match decide (lm_is_stopped ρlg δ) with
+    | left STOP => Some (reset_lm_st_impl ρlg δ STOP)
+    | _ => None
+    end.
+
+  Definition reset_lm_st_rel ρlg: relation (fmstate lib_fair) :=
+    fun x y => reset_lm_st ρlg x = Some y.
+
+  Inductive lib_lm_EI := eiG (ρlg: lib_grole).
+
+  Instance lib_lm_EI_eqdec: EqDecision lib_lm_EI.
+  Proof. solve_decision. Qed. 
+
+  Instance lib_lm_EI_cnt: Countable lib_lm_EI.
+  Proof.
+    apply inj_countable' with
+      (f := fun ι => match ι with | eiG ρlg => ρlg end)
+      (g := eiG).
+    intros. by destruct x. 
+  Qed.  
+
+  (* TODO: avoid duplication *)
+  Definition lib_lm_active_exts (δ: fmstate lib_fair): gset lib_lm_EI := 
+    set_map eiG $ filter (flip lm_is_stopped δ) (dom (ls_tmap δ (LM := lib_model))). 
+  
+  Definition lib_lm_ETs '(eiG ρlg) := reset_lm_st_rel ρlg. 
+
+  (* TODO: move, find existing? *)
+  Lemma iff_and_impl_helper {A B: Prop} (AB: A -> B):
+    A /\ B <-> A.
+  Proof. tauto. Qed.     
+  Lemma iff_True_helper {A: Prop}:
+    (A <-> True) <-> A.
+  Proof. tauto. Qed.     
+  Lemma iff_False_helper {A: Prop}:
+    (A <-> False) <-> ¬ A.
+  Proof. tauto. Qed.
+
+  Let lib_lm_projEI (_: lib_lm_EI) := (tt: lib_EI).
+
+  Lemma lib_lm_active_exts_spec:
+    ∀ δ ι, ι ∈ lib_lm_active_exts δ ↔ (∃ δ' : lib_fair, lib_lm_ETs ι δ δ'). 
+  Proof using.
+    intros. 
+    destruct ι. simpl.
+    rewrite /lib_lm_active_exts /reset_lm_st_rel /reset_lm_st.
+    erewrite <- set_map_properties.elem_of_map_inj_gset.
+    2: { red. by intros ??[=]. }
+    rewrite elem_of_filter. simpl.
+    rewrite iff_and_impl_helper.
+    2: { rewrite /lm_is_stopped. tauto. }
+    destruct decide.
+    - transitivity True; [tauto| ].
+      symmetry. apply iff_True_helper. eauto.
+    - transitivity False; [tauto| ].
+      symmetry. apply iff_False_helper.
+      by intros [??].
+  Qed.
+
+  Definition ExtLibLM: ExtModel (LM_Fair (LM := lib_model)) :=
+    Build_ExtModel (LM_Fair (LM := lib_model)) _ _ _ _ _ lib_lm_active_exts_spec. 
+
+
+End ExtModelLM. 
